Find the general solution to the original ODE.

\nl Using the $M$ and $N$ from part (c), integrating for $\int M \dd x$ and $\int N \dd y$ gives
\begin{align*}
    \int M \dd x && \int N \dd y \\
    \int -2xy^{-3} \dd x && \int 3x^2 y^{-4} - y^{-2} \dd y\\
    -x^2 y^{-3} + C(y) && -x^2y^{-3} + y^{-1} + C(x).
\end{align*}
Therefore $C(y) = y^{-1} + C$ and $C(x) = 0$. Hence, $f(x,y) = -x^2y^{-3} + y^{-1} + C$.
This solution can be verified as follows,
\begin{align*}
    & \dv{x} \Bigbrac{ -x^2y^{-3} + y^{-1} = -C} \\
    & 3x^2y^{-4}y' - 2xy^{-3} -y^{-2}y' = 0\\
    & y' = \frac{2xy^{-3}}{3x^2y^{-4}-y^{-2}}\\
    & y' = \frac{2xy^2}{3x-y^2} = \dv{y}{x}\\
\end{align*}