Since $A = P$ and
\begin{align*}
    S &= PDP^{-1}\\
    &=  \begin{bmatrix}
        1&0&0&0\\
        0&1&0&0\\
        0&0&\frac{i\sqrt{2}}{2} & - \frac{i\sqrt{2}}{2} \\
        0&0&1&1
        \end{bmatrix} \begin{bmatrix}
        2 &0&0&0\\
        0&2&0&0\\
        0&0&2 + i \sqrt{2}&0\\
        0&0&0&2 - i \sqrt{2}
    \end{bmatrix}
    \begin{bmatrix}
        1&0&0&0\\
        0&1&0&0\\
        0&0&-\frac{i\sqrt{2}}{2} & \frac{1}{2}\\
        0&0&\frac{i\sqrt{2}}{2}&\frac{1}{2}
        \end{bmatrix}\\
        &= \begin{bmatrix}
            2&0&&\\
            0&2&&\\
            &&2&-2\\
            &&2&2
        \end{bmatrix}
\end{align*}
Then $N = A-S = \begin{bmatrix}
    0&1&0&0\\
    &0&0&0\\
    &&0&0\\
    &&&0
\end{bmatrix}$ which is clearly nilpotent of degree 2. Then $e^{At} = e^{(S+N)t} = e^{St}.e^{Nt}$. By the exponential definition we know $e^{Nt} = I + Nt + 0 +  \dots = \begin{bmatrix}
    1&t&0&0\\
    &1&0&0\\
    &&1&0\\
    &&&1
\end{bmatrix}$. Then reverse-engineering the notes, $e^{St} = \begin{bmatrix}
    e^{2t} & 0 & & \\
    0&e^{2t}&&\\
    &&e^{2t} \cos(2t) & -e^{2t}\sin(2t)\\
    &&e^{2t}\sin(2t) & e^{2t} \cos(2t) 
\end{bmatrix}$. Lastly $e^{At} = e^{St}.e^{Nt} = e^{Nt}.e^{St}$ which is 
$$e^{At} =  \begin{bmatrix}
    e^{2t} & te^{2t} & & \\
    0&e^{2t}&&\\
    &&e^{2t} \cos(2t) & -e^{2t}\sin(2t)\\
    &&e^{2t}\sin(2t) & e^{2t} \cos(2t) 
\end{bmatrix}$$