Since $A = PJP^{-1}$ then certainly $P^{-1}AP = J$. Hence
\begin{align*}
    J
    &= P^{-1}AP\\
    &= \frac{1}{10}\begin{bmatrix}
        1&1&1&1\\
        2&-8&2&2\\
        3&3&-7&3\\
        4&4&4&-6
    \end{bmatrix}  
    \begin{bmatrix}
        1&1&1&1 \\ 2&2&2&2 \\ 3&3&3&3 \\ 4&4&4&4
    \end{bmatrix}
    \begin{bmatrix}
        1 & 1 & 1 & 1\\
        2&-1&0&0\\
        3&0&-1&0\\
        4&0&0&-1
    \end{bmatrix}\\
    &=
    \begin{bmatrix*}
        10&0& 0 & 0 \\
        0&0&0&0\\
        0&0&0&0 \\
        0&0&0&0
    \end{bmatrix*}
\end{align*}